SystemF2Data: cleanups
Ignore-this: 908504bea1a13e4c772c7c095f59d502

darcs-hash:20130425124821-08f32-dfd53029fb2ae0de5ad3a580501bd9cae5df81c6

done/Iron/Language/SystemF2Data/Type/Exp.v
@@ -21,4 +21,8 @@ Definition tFun (t1: ty) (t2: ty)
  := TApp (TApp (TCon TyConFun) t1) t2.
 Hint Unfold tFun.
 
+Definition tNat
+ := TCon TyConNat.
 
+Definition tBool
+ := TCon TyConBool.
