done/Iron/Language/SystemF2Data/Exp/Relation/WnfX.v
@@ -3,6 +3,7 @@ Require Export Iron.Language.SystemF2Data.Exp.Base.
 Require Export Iron.Language.SystemF2Data.Exp.Relation.WfX.
 
 
+(********************************************************************)
 (* Weak normal forms cannot be reduced further by 
    call-by-value evaluation. *)
 Inductive wnfX : exp -> Prop :=
@@ -29,6 +30,7 @@ Inductive wnfX : exp -> Prop :=
 Hint Constructors wnfX.
 
 
+(********************************************************************)
 (* Values are closed expressions that cannot be reduced further. *)
 Inductive value : exp -> Prop :=
  | Value 
